coq/NNRSimp/Optim/NNRSimpUnflatten.v
@@ -1,0 +1,669 @@
+(*
+ * Copyright 2015-2016 IBM Corporation
+ *
+ * Licensed under the Apache License, Version 2.0 (the "License");
+ * you may not use this file except in compliance with the License.
+ * You may obtain a copy of the License at
+ *
+ * http://www.apache.org/licenses/LICENSE-2.0
+ *
+ * Unless required by applicable law or agreed to in writing, software
+ * distributed under the License is distributed on an "AS IS" BASIS,
+ * WITHOUT WARRANTIES OR CONDITIONS OF ANY KIND, either express or implied.
+ * See the License for the specific language governing permissions and
+ * limitations under the License.
+ *)
+
+(* This includes some rewrites/simplification rules for the Nested relational calculus *)
+
+Require Import String.
+Require Import List.
+Require Import ListSet.
+Require Import Arith.
+Require Import Bool.
+Require Import Equivalence.
+Require Import Morphisms.
+Require Import Setoid.
+Require Import Decidable.
+Require Import EquivDec.
+Require Import Program.
+Require Import Utils.
+Require Import CommonRuntime.
+Require Import NNRSimpRuntime.
+
+Section NNRSimpUnflatten.
+  Local Open Scope nnrs_imp.
+
+  Context {fruntime:foreign_runtime}.
+
+  Section unflatten.
+    (* This should really be done via (backwards propagating) dataflow analysis, 
+     but we don't currently have a dataflow analysis set up. 
+     For a single variable, this should work; although it will not see through
+     assignments *)
+
+    Section def.
+
+      Fixpoint nnrs_imp_expr_unflatten_init (e:nnrs_imp_expr) : option nnrs_imp_expr
+        := match e with
+           | NNRSimpBinop OpBagUnion e₁ e₂ =>
+             lift2 (NNRSimpBinop OpBagUnion)
+                   (nnrs_imp_expr_unflatten_init e₁)
+                   (nnrs_imp_expr_unflatten_init e₂)
+           | NNRSimpUnop OpBag (NNRSimpConst (dcoll l)) =>
+             Some (NNRSimpConst (dcoll l))
+           | NNRSimpUnop OpBag (NNRSimpUnop OpBag e₁) =>
+             Some (NNRSimpUnop OpBag e₁)
+           | NNRSimpConst (dcoll nil) =>
+             Some (NNRSimpConst (dcoll nil))
+           | NNRSimpConst (dcoll ((dcoll l)::nil)) =>
+             Some (NNRSimpConst (dcoll l))
+           | _ => None
+           end.
+
+      Definition nnrs_imp_expr_unflatten_init_option (oe:option nnrs_imp_expr) 
+        : option (option nnrs_imp_expr)
+        := match oe with
+           | Some e => lift Some (nnrs_imp_expr_unflatten_init e)
+           | None => Some None
+           end.
+
+      Fixpoint nnrs_imp_expr_unflatten_read (e:nnrs_imp_expr) (v:var) : option nnrs_imp_expr
+        := match e with
+           | NNRSimpVar x =>
+             if x == v
+             then None
+             else Some (NNRSimpVar x)
+           | NNRSimpUnop OpFlatten (NNRSimpVar x) =>
+             if x == v
+             then Some (NNRSimpVar x)
+             else Some (NNRSimpUnop OpFlatten (NNRSimpVar x) )
+           | NNRSimpGetConstant x =>
+             Some (NNRSimpGetConstant x)
+           | NNRSimpConst d =>
+             Some (NNRSimpConst d)
+           | NNRSimpUnop u e₁ =>
+             lift (NNRSimpUnop u)
+                  (nnrs_imp_expr_unflatten_read e₁ v)
+           | NNRSimpBinop b e₁ e₂ =>
+             lift2 (NNRSimpBinop b)
+                   (nnrs_imp_expr_unflatten_read e₁ v)
+                   (nnrs_imp_expr_unflatten_read e₂ v)
+           | NNRSimpGroupBy g sl e₁ =>
+             lift (NNRSimpGroupBy g sl) (nnrs_imp_expr_unflatten_read e₁ v)
+           end.
+
+      Definition nnrs_imp_expr_unflatten_read_option (oe:option nnrs_imp_expr) (v:var)
+        : option (option nnrs_imp_expr)
+        := match oe with
+           | Some e => lift Some (nnrs_imp_expr_unflatten_read e v)
+           | None => Some None
+           end.
+
+      Fixpoint nnrs_imp_expr_unflatten_write (e:nnrs_imp_expr) (v:var) : option nnrs_imp_expr
+        := match e with
+           | NNRSimpVar x =>
+             if x == v
+             then Some (NNRSimpVar x)
+             else None
+           | NNRSimpBinop OpBagUnion e₁ e₂ =>
+             lift2 (NNRSimpBinop OpBagUnion)
+                   (nnrs_imp_expr_unflatten_write e₁ v)
+                   (nnrs_imp_expr_unflatten_write e₂ v)
+           | NNRSimpUnop OpBag e₁ =>
+             if in_dec string_dec v (nnrs_imp_expr_free_vars e₁)
+             then None
+             else Some e₁
+           | NNRSimpConst (dcoll nil) =>
+             Some (NNRSimpConst (dcoll nil))
+           | NNRSimpConst (dcoll ((dcoll l)::nil)) =>
+             Some (NNRSimpConst (dcoll l))
+           | _ => None
+           end.
+
+      Definition lift3 {A B C D} (f:A->B->C->D) x y z
+        := match x, y, z with
+           | Some x, Some y, Some z => Some (f x y z)
+           | _, _, _ => None
+           end.
+      
+      Fixpoint nnrs_imp_stmt_unflatten (s:nnrs_imp_stmt) (v:var) : option nnrs_imp_stmt
+        := match s with
+           | NNRSimpSkip =>
+             Some NNRSimpSkip
+           | NNRSimpSeq s₁ s₂ =>
+             lift2 NNRSimpSeq
+                   (nnrs_imp_stmt_unflatten s₁ v)
+                   (nnrs_imp_stmt_unflatten s₂ v)
+           | NNRSimpAssign x e =>
+             lift (NNRSimpAssign x)
+                  (if x == v
+                   then nnrs_imp_expr_unflatten_write e v
+                   else nnrs_imp_expr_unflatten_read e v)
+           | NNRSimpLet x oe s₁ =>
+             lift2 (NNRSimpLet x)
+                   (nnrs_imp_expr_unflatten_read_option oe v)
+                   (if x == v then Some s₁ else nnrs_imp_stmt_unflatten s₁ v)
+           | NNRSimpFor x e s₁ =>
+             lift2 (NNRSimpFor x)
+                   (nnrs_imp_expr_unflatten_read e v)
+                   (if x == v then Some s₁ else nnrs_imp_stmt_unflatten s₁ v)
+           | NNRSimpIf e s₁ s₂ =>
+             lift3 NNRSimpIf
+                   (nnrs_imp_expr_unflatten_read e v)
+                   (nnrs_imp_stmt_unflatten s₁ v)
+                   (nnrs_imp_stmt_unflatten s₂ v)
+           | NNRSimpEither e x₁ s₁ x₂ s₂ =>
+             lift3 (fun e s₁ s₂ => NNRSimpEither e x₁ s₁ x₂ s₂)
+                   (nnrs_imp_expr_unflatten_read e v)
+                   (if x₁ == v then Some s₁ else nnrs_imp_stmt_unflatten s₁ v)
+                   (if x₂ == v then Some s₂ else nnrs_imp_stmt_unflatten s₂ v)
+           end.
+
+      Section safe.
+
+        Fixpoint nnrs_imp_stmt_read_out (s:nnrs_imp_stmt) (v:var) : bool
+          := match s with
+             | NNRSimpSkip => false
+             | NNRSimpSeq s₁ s₂ =>
+               nnrs_imp_stmt_read_out s₁ v
+               || nnrs_imp_stmt_read_out s₂ v
+             | NNRSimpAssign x e =>
+               (x <>b v) && nnrs_imp_expr_may_use e v
+             | NNRSimpLet x oe s₁ =>
+               match oe with
+               | Some e => nnrs_imp_expr_may_use e v
+               | None => false
+               end
+               || ((x <>b v) && nnrs_imp_stmt_read_out s₁ v)
+             | NNRSimpFor x e s₁ =>
+               nnrs_imp_expr_may_use e v
+               || ((x <>b v) && nnrs_imp_stmt_read_out s₁ v)
+             | NNRSimpIf e s₁ s₂ =>
+               nnrs_imp_expr_may_use e v
+               || nnrs_imp_stmt_read_out s₁ v
+               || nnrs_imp_stmt_read_out s₂ v
+             | NNRSimpEither e x₁ s₁ x₂ s₂ =>
+               nnrs_imp_expr_may_use e v
+               || ((x₁ <>b v) && nnrs_imp_stmt_read_out s₁ v)
+               || ((x₂ <>b v) && nnrs_imp_stmt_read_out s₂ v)
+             end.
+        
+        Definition nnrs_imp_stmt_unflatten_safe s v : option nnrs_imp_stmt
+          := if nnrs_imp_stmt_read_out s v
+             then nnrs_imp_stmt_unflatten s v
+             else None.
+
+      End safe.
+
+    End def.
+
+    Section ident.
+      
+      Lemma nnrs_imp_expr_unflatten_read_nfree_id {e v}:
+        ~ In v (nnrs_imp_expr_free_vars e) ->
+        nnrs_imp_expr_unflatten_read e v = Some e.
+      Proof.
+        nnrs_imp_expr_cases (induction e) Case
+        ; simpl; intros nfree
+        ; trivial.
+        - Case "NNRSimpVar"%string.
+          match_destr.
+          tauto.
+        - Case "NNRSimpBinop"%string.
+          rewrite in_app_iff in *.
+          rewrite IHe1, IHe2; tauto.
+        - Case "NNRSimpUnop"%string.
+          rewrite IHe by tauto.
+          destruct u; simpl; try reflexivity.
+          destruct e; simpl; try reflexivity.
+          destruct (equiv_dec v0 v); try reflexivity.
+          simpl in *; tauto.
+        - Case "NNRSimpGroupBy"%string.
+          rewrite IHe; tauto.
+      Qed.
+
+      Lemma nnrs_imp_stmt_unflatten_nfree_id {s v}:
+        ~ In v (nnrs_imp_stmt_free_vars s) ->
+        nnrs_imp_stmt_unflatten s v = Some s.
+      Proof.
+        nnrs_imp_stmt_cases (induction s) Case
+        ; simpl; repeat rewrite in_app_iff; intros nfree
+        ; trivial.
+        - Case "NNRSimpSeq"%string.
+          rewrite IHs1, IHs2; eauto.
+        - Case "NNRSimpAssign"%string.
+          match_destr; try tauto.
+          rewrite nnrs_imp_expr_unflatten_read_nfree_id; tauto.
+        - Case "NNRSimpLet"%string.
+          destruct o; simpl.
+          + rewrite nnrs_imp_expr_unflatten_read_nfree_id by tauto.
+            simpl.
+            destruct (equiv_dec v0 v); trivial.
+            rewrite IHs; intuition.
+            apply remove_nin_inv in H1.
+            intuition.
+          + destruct (equiv_dec v0 v); trivial.
+            rewrite IHs; intuition.
+            apply remove_nin_inv in H1.
+            intuition.
+        - Case "NNRSimpFor"%string.
+          rewrite nnrs_imp_expr_unflatten_read_nfree_id by tauto.
+          destruct (equiv_dec v0 v); trivial.
+          rewrite IHs; intuition.
+          apply remove_nin_inv in H1.
+          intuition.
+        - Case "NNRSimpIf"%string.
+          rewrite nnrs_imp_expr_unflatten_read_nfree_id by tauto.
+          rewrite IHs1, IHs2; tauto.
+        - Case "NNRSimpEither"%string.
+          rewrite nnrs_imp_expr_unflatten_read_nfree_id by tauto.
+          simpl; intuition.
+          apply remove_nin_inv in H1.
+          apply remove_nin_inv in H2.
+          destruct (equiv_dec v0 v); trivial
+          ; destruct (equiv_dec v1 v); trivial.
+          + rewrite IHs2; intuition.
+          + rewrite IHs1; intuition congruence.
+          + rewrite IHs1, IHs2; intuition congruence.
+      Qed.
+
+    End ident.
+    Section eval.
+
+      Definition flattens_to (d d':data)
+        := match d, d' with
+           | dcoll l, dcoll l' => oflatten l = Some l'
+           | _, _ => False
+           end.
+
+      Definition flattens_to_op (d d':data)
+        : flattens_to d d'
+          <-> lift_oncoll (fun l => (lift dcoll (oflatten l))) d = Some d'.
+      Proof.
+        destruct d; simpl
+        ; try (intuition congruence).
+        destruct d'; simpl
+        ; try solve [destruct (oflatten l); simpl; try intuition congruence].
+      Qed.
+
+      Lemma nnrs_imp_expr_unflatten_init_eval e e' h σc σ :
+        nnrs_imp_expr_unflatten_init e = Some e' ->
+        lift2P flattens_to
+               (nnrs_imp_expr_eval h σc σ e)
+               (nnrs_imp_expr_eval h σc σ e').
+      Proof.
+        revert e'.
+        nnrs_imp_expr_cases (induction e) Case
+        ; simpl ; intros e' eqq
+        ; try discriminate.
+        - Case "NNRSimpConst"%string.
+          destruct d; simpl in *
+          ; invcs eqq.
+          destruct l; invcs H0; simpl.
+          + reflexivity.
+          + destruct d; invcs H1.
+            destruct l; invcs H0.
+            simpl.
+            unfold oflatten; simpl.
+            rewrite app_nil_r; trivial.
+        - Case "NNRSimpBinop"%string.
+          destruct b; try discriminate.
+          apply some_lift2 in eqq.
+          destruct eqq as [?[? eqq1[eqq2 ?]]]; subst.
+          specialize (IHe1 _ eqq1).
+          specialize (IHe2 _ eqq2).
+          unfold lift2P in *; simpl.
+          repeat match_option_in IHe1
+          ; simpl in *
+          ; try contradiction.
+          repeat match_option_in IHe2
+          ; simpl in *
+          ; try contradiction.
+
+          destruct d; simpl in *; try contradiction
+          ; destruct d0; simpl in *; try contradiction
+          ; trivial
+          ; destruct d1; simpl in *; try contradiction
+          ; destruct d2; simpl in *; try contradiction
+          ; trivial.
+          unfold bunion.
+          apply oflatten_app; trivial.
+        - Case "NNRSimpUnop"%string.
+          destruct u; simpl; try discriminate.
+          destruct e; simpl; try discriminate.
+          + destruct d; simpl; try discriminate.
+            invcs eqq; simpl.
+            unfold oflatten, lift_flat_map; simpl.
+            rewrite app_nil_r; trivial.
+          + destruct u; simpl; try discriminate.
+            invcs eqq; simpl.
+            destruct (nnrs_imp_expr_eval h σc σ e); simpl; trivial.
+      Qed.
+
+      Lemma nnrs_imp_expr_unflatten_read_eval e e' v h σc σ d d' :
+        nnrs_imp_expr_unflatten_read e v = Some e' ->
+        lookup equiv_dec σ v = Some d ->
+        lift2P flattens_to d d' ->
+        nnrs_imp_expr_eval h σc σ e =
+        nnrs_imp_expr_eval h σc (update_first equiv_dec σ v d') e'.
+      Proof.
+        revert e' d d'.
+        nnrs_imp_expr_cases (induction e) Case
+        ; simpl ; intros e' dd dd' eqq inn ft
+        ; try discriminate.
+        - Case "NNRSimpGetConstant"%string.
+          invcs eqq; simpl; trivial.
+        - Case "NNRSimpVar"%string.
+          match_destr_in eqq.
+          invcs eqq; simpl.
+          rewrite lookup_update_neq; trivial.
+          eauto.
+        - Case "NNRSimpConst"%string.
+          invcs eqq; simpl; trivial.
+        - Case "NNRSimpBinop"%string.
+          apply some_lift2 in eqq.
+          destruct eqq as [?[? eqq1[eqq2 ?]]]; subst.
+          simpl.
+          erewrite IHe1, IHe2; eauto.
+        - Case "NNRSimpUnop"%string.
+          destruct u
+          ; try solve [apply some_lift in eqq
+                       ; destruct eqq as [eqq1 eqq2]
+                       ; subst; simpl
+                       ; erewrite IHe; eauto].
+          destruct e
+          ; try solve [apply some_lift in eqq
+                       ; destruct eqq as [eqq1 eqq2]
+                       ; subst; simpl in *
+                       ; invcs eqq2
+                       ; simpl; trivial
+                       ; erewrite IHe; eauto].
+          match_destr_in eqq.
+          + invcs eqq; simpl.
+            rewrite e.
+            rewrite lookup_update_eq_in.
+            * unfold var in *. rewrite inn; simpl.
+              unfold id.
+              unfold lift2P in ft.
+              repeat match_destr_in ft; simpl; try contradiction.
+              apply flattens_to_op; trivial.
+            * apply lookup_in_domain in inn; trivial.
+          + invcs eqq; simpl.
+            rewrite lookup_update_neq; eauto.
+        - Case "NNRSimpGroupBy"%string.
+          apply some_lift in eqq.
+          destruct eqq as [??]; subst; simpl.
+          erewrite IHe; eauto.
+      Qed.              
+
+    End eval.
+
+    
+    Section free_vars.
+      
+      Lemma nnrs_imp_expr_unflatten_init_free_vars e e' :
+        nnrs_imp_expr_unflatten_init e = Some e' ->
+        nnrs_imp_expr_free_vars e = nnrs_imp_expr_free_vars e'.
+      Proof.
+        revert e'.
+        nnrs_imp_expr_cases (induction e) Case
+        ; simpl ; intros e' eqq
+        ; try discriminate.
+        - Case "NNRSimpConst"%string.
+          destruct d; simpl in *
+          ; invcs eqq.
+          destruct l; simpl in *.
+          + invcs H0; simpl; trivial.
+          + destruct d; simpl; try discriminate.
+            destruct l; simpl; try discriminate.
+            invcs H0.
+            simpl; trivial.
+        - Case "NNRSimpBinop"%string.
+          destruct b; try discriminate.
+          apply some_lift2 in eqq.
+          destruct eqq as [?[? eqq1[eqq2 ?]]]; subst.
+          erewrite IHe1 by eauto.
+          erewrite IHe2 by eauto.
+          simpl; congruence.
+        - Case "NNRSimpUnop"%string.
+          destruct u; try discriminate.
+          destruct e; try discriminate.
+          + destruct d; try discriminate.
+            invcs eqq; trivial.
+          + destruct u; try discriminate.
+            invcs eqq.
+            simpl; trivial.
+      Qed.
+      
+      Lemma nnrs_imp_expr_unflatten_read_free_vars e e' v :
+        nnrs_imp_expr_unflatten_read e v = Some e' ->
+        nnrs_imp_expr_free_vars e = nnrs_imp_expr_free_vars e'.
+      Proof.
+        revert e'
+        ; nnrs_imp_expr_cases (induction e) Case
+        ; simpl ; intros e' eqq
+        ; try discriminate.
+        - Case "NNRSimpGetConstant"%string.
+          invcs eqq; simpl; trivial.
+        - Case "NNRSimpVar"%string.
+          match_destr_in eqq.
+          invcs eqq; simpl; trivial.
+        - Case "NNRSimpConst"%string.
+          invcs eqq; simpl; trivial.
+        - Case "NNRSimpBinop"%string.
+          apply some_lift2 in eqq.
+          destruct eqq as [?[? eqq1[eqq2 ?]]]; subst.
+          erewrite IHe1 by eauto.
+          erewrite IHe2 by eauto.
+          simpl; congruence.
+        - Case "NNRSimpUnop"%string.
+          destruct u
+          ; try solve [apply some_lift in eqq
+                       ; destruct eqq as [? eqq1 ?]; subst
+                       ; erewrite IHe by eauto; simpl; trivial].
+          destruct e
+          ; try solve [apply some_lift in eqq
+                       ; destruct eqq as [? eqq1 ?]; subst
+                       ; erewrite IHe by eauto; simpl; trivial].
+          match_destr_in eqq.
+          + invcs eqq; trivial.
+          + invcs eqq; trivial.
+        - Case "NNRSimpGroupBy"%string.
+          apply some_lift in eqq
+          ; destruct eqq as [? eqq1 ?]; subst
+          ; erewrite IHe by eauto; simpl; trivial.
+      Qed.
+
+      Lemma nnrs_imp_expr_unflatten_write_free_vars e e' v :
+        nnrs_imp_expr_unflatten_write e v = Some e' ->
+        nnrs_imp_expr_free_vars e = nnrs_imp_expr_free_vars e'.
+      Proof.
+        revert e'
+        ; nnrs_imp_expr_cases (induction e) Case
+        ; simpl ; intros e' eqq
+        ; try discriminate.
+        - Case "NNRSimpVar"%string.
+          match_destr_in eqq.
+          invcs eqq; simpl; trivial.
+        - Case "NNRSimpConst"%string.
+          destruct d; simpl in *
+          ; invcs eqq.
+          destruct l; simpl in *.
+          + invcs H0; simpl; trivial.
+          + destruct d; simpl; try discriminate.
+            destruct l; simpl; try discriminate.
+            invcs H0.
+            simpl; trivial.
+        - Case "NNRSimpBinop"%string.
+          destruct b; simpl; try discriminate.
+          apply some_lift2 in eqq.
+          destruct eqq as [?[? eqq1[eqq2 ?]]]; subst.
+          erewrite IHe1 by eauto.
+          erewrite IHe2 by eauto.
+          simpl; congruence.
+        - Case "NNRSimpUnop"%string.
+          destruct u; try discriminate.
+          match_destr_in eqq.
+          invcs eqq; trivial.
+      Qed.
+
+      Lemma nnrs_imp_stmt_unflatten_free_vars s s' v :
+        nnrs_imp_stmt_unflatten s v = Some s' ->
+        nnrs_imp_stmt_free_vars s = nnrs_imp_stmt_free_vars s'.
+      Proof.
+        revert s'
+        ; nnrs_imp_stmt_cases (induction s) Case
+        ; simpl ; intros s' eqq.
+        - Case "NNRSimpSkip"%string.
+          invcs eqq; simpl; trivial.
+        - Case "NNRSimpSeq"%string.
+          apply some_lift2 in eqq.
+          destruct eqq as [?[? eqq1[eqq2 ?]]]; subst.
+          erewrite IHs1 by eauto.
+          erewrite IHs2 by eauto.
+          simpl; congruence.
+        - Case "NNRSimpAssign"%string.
+          apply some_lift in eqq.
+          destruct eqq as [? eqq ?]; subst.
+          match_destr_in eqq; simpl.
+          + eapply nnrs_imp_expr_unflatten_write_free_vars in eqq; congruence.
+          + eapply nnrs_imp_expr_unflatten_read_free_vars in eqq; congruence.
+        - Case "NNRSimpLet"%string.
+          apply some_lift2 in eqq.
+          destruct eqq as [?[? eqq1[eqq2 ?]]]; subst.
+          simpl.
+          f_equal.
+          + destruct o; simpl in *.
+            * apply some_lift in eqq1.
+              destruct eqq1 as [? eqq1 ?]; subst.
+              eapply nnrs_imp_expr_unflatten_read_free_vars in eqq1; congruence.
+            * invcs eqq1; trivial.
+          + match_destr_in eqq2.
+            * invcs eqq2; trivial.
+            * eapply IHs in eqq2; congruence.
+        - Case "NNRSimpFor"%string.
+          apply some_lift2 in eqq.
+          destruct eqq as [?[? eqq1[eqq2 ?]]]; subst.
+          simpl.
+          eapply nnrs_imp_expr_unflatten_read_free_vars in eqq1.
+          f_equal; trivial.
+          match_destr_in eqq2.
+          + invcs eqq2; trivial.
+          + eapply IHs in eqq2; congruence.
+        - Case "NNRSimpIf"%string.
+          unfold lift3 in eqq.
+          repeat match_option_in eqq.
+          invcs eqq.
+          simpl.
+          eapply nnrs_imp_expr_unflatten_read_free_vars in eqq0.
+          rewrite eqq0.
+          f_equal.
+          f_equal; eauto.
+        - Case "NNRSimpEither"%string.
+          unfold lift3 in eqq.
+          repeat match_option_in eqq.
+          invcs eqq.
+          simpl.
+          eapply nnrs_imp_expr_unflatten_read_free_vars in eqq0.
+          rewrite eqq0.
+          f_equal.
+          f_equal.
+          + match_destr_in eqq1.
+            * invcs eqq1; trivial.
+            * eapply IHs1 in eqq1; congruence.
+          + match_destr_in eqq2.
+            * invcs eqq2; trivial.
+            * eapply IHs2 in eqq2; congruence.
+      Qed.
+
+    End free_vars.
+
+    Section usage.
+
+      Lemma nnrs_imp_stmt_unflatten_var_usage {s s' v}:
+        nnrs_imp_stmt_unflatten s v = Some s' ->
+        forall v',
+          nnrs_imp_stmt_var_usage s v' = nnrs_imp_stmt_var_usage s' v'.
+      Proof.
+        revert s'
+        ; nnrs_imp_stmt_cases (induction s) Case
+        ; simpl ; intros s' eqq v'.
+        - Case "NNRSimpSkip"%string.
+          invcs eqq; simpl; trivial.
+        - Case "NNRSimpSeq"%string.
+          apply some_lift2 in eqq.
+          destruct eqq as [?[? eqq1[eqq2 ?]]]; subst.
+          erewrite IHs1 by eauto.
+          erewrite IHs2 by eauto.
+          simpl; congruence.
+        - Case "NNRSimpAssign"%string.
+          apply some_lift in eqq.
+          destruct eqq as [? eqq ?]; subst.
+          match_destr_in eqq; simpl.
+          + eapply nnrs_imp_expr_unflatten_write_free_vars in eqq.
+            rewrite (nnrs_imp_expr_may_use_free_vars_eq eqq); trivial.
+          + eapply nnrs_imp_expr_unflatten_read_free_vars in eqq.
+            rewrite (nnrs_imp_expr_may_use_free_vars_eq eqq); trivial.
+        - Case "NNRSimpLet"%string.
+          apply some_lift2 in eqq.
+          destruct eqq as [?[? eqq1[eqq2 ?]]]; subst.
+          destruct o; simpl in *.
+          + apply some_lift in eqq1.
+            destruct eqq1 as [? eqq1 ?]; subst.
+            eapply nnrs_imp_expr_unflatten_read_free_vars in eqq1.
+            rewrite (nnrs_imp_expr_may_use_free_vars_eq eqq1); trivial.
+            match_destr.
+            unfold equiv_decb.
+            match_destr_in eqq2.
+            * invcs eqq2; trivial.
+            * rewrite (IHs _ eqq2); trivial.
+          + invcs eqq1.
+            unfold equiv_decb.
+            match_destr_in eqq2.
+            * invcs eqq2; trivial.
+            * rewrite (IHs _ eqq2); trivial.
+        - Case "NNRSimpFor"%string.
+          apply some_lift2 in eqq.
+          destruct eqq as [?[? eqq1[eqq2 ?]]]; subst.
+          simpl.
+          eapply nnrs_imp_expr_unflatten_read_free_vars in eqq1.
+          rewrite (nnrs_imp_expr_may_use_free_vars_eq eqq1); trivial.
+          match_destr.
+          unfold equiv_decb.
+          match_destr_in eqq2.
+          * invcs eqq2; trivial.
+          * rewrite (IHs _ eqq2); trivial.
+        - Case "NNRSimpIf"%string.
+          unfold lift3 in eqq.
+          repeat match_option_in eqq.
+          invcs eqq; simpl.
+          eapply nnrs_imp_expr_unflatten_read_free_vars in eqq0.
+          rewrite (nnrs_imp_expr_may_use_free_vars_eq eqq0); trivial.
+          match_destr.
+          rewrite (IHs1 _ eqq1).
+          rewrite (IHs2 _ eqq2).
+          trivial.
+        - Case "NNRSimpEither"%string.
+          unfold lift3 in eqq.
+          repeat match_option_in eqq.
+          invcs eqq; simpl.
+          eapply nnrs_imp_expr_unflatten_read_free_vars in eqq0.
+          rewrite (nnrs_imp_expr_may_use_free_vars_eq eqq0); trivial.
+          match_destr.
+          match_destr_in eqq1.                         
+          + invcs eqq1.
+            match_destr_in eqq2.
+            * invcs eqq2; trivial.
+            * rewrite (IHs2 _ eqq2); trivial.
+          + rewrite (IHs1 _ eqq1).
+            match_destr_in eqq2.
+            * invcs eqq2; trivial.
+            * rewrite (IHs2 _ eqq2); trivial.
+      Qed.
+
+    End usage.
+    
+  End unflatten.
+  
+End NNRSimpUnflatten.
