coq/NNRSimp/Optim/TNNRSimpUnflatten.v
@@ -1,0 +1,1161 @@
+(*
+ * Copyright 2015-2016 IBM Corporation
+ *
+ * Licensed under the Apache License, Version 2.0 (the "License");
+ * you may not use this file except in compliance with the License.
+ * You may obtain a copy of the License at
+ *
+ * http://www.apache.org/licenses/LICENSE-2.0
+ *
+ * Unless required by applicable law or agreed to in writing, software
+ * distributed under the License is distributed on an "AS IS" BASIS,
+ * WITHOUT WARRANTIES OR CONDITIONS OF ANY KIND, either express or implied.
+ * See the License for the specific language governing permissions and
+ * limitations under the License.
+ *)
+
+(* This includes some rewrites/simplification rules for the Nested relational calculus *)
+
+Require Import String.
+Require Import List.
+Require Import ListSet.
+Require Import Arith.
+Require Import Bool.
+Require Import Morphisms.
+Require Import Setoid.
+Require Import Decidable.
+Require Import EquivDec.
+Require Import Equivalence.
+Require Import Program.
+Require Import Utils.
+Require Import CommonSystem.
+Require Import NNRSimpSystem.
+Require Import NNRSimpUnflatten.
+
+Section TNNRSimpUnflatten.
+  Local Open Scope nnrs_imp.
+
+  Context {m:basic_model}.
+
+  Hint Immediate type_NNRSimpSkip.
+
+
+  Section eval.
+    (* these evaluation lemmas require the Coll (Coll constraint).
+       We could probably write them via checking the shape of the 
+       evaluated data instead, but since we ultimately care about 
+       well-typed expresions anyway, this seems more straightforward.
+     *)
+    Lemma nnrs_imp_expr_unflatten_write_eval e e' v σc σ :
+      nnrs_imp_expr_unflatten_write e v = Some e' ->
+      forall Γc,
+        bindings_type σc Γc ->
+        forall Γ,
+          pd_bindings_type σ Γ ->
+          forall τ,
+            [ Γc ; Γ  ⊢ e ▷ Coll (Coll τ) ] ->
+            forall d d',
+            lookup equiv_dec σ v = Some d ->
+        lift2P flattens_to d d' ->
+        lift2P
+          flattens_to
+          (nnrs_imp_expr_eval brand_relation_brands σc σ e)
+          (nnrs_imp_expr_eval brand_relation_brands σc (update_first equiv_dec σ v d') e').
+      Proof.
+        intros eqq Γc Γc_bt Γ Γ_bt  τ typ d d' inn ft.
+        revert e' eqq typ.
+        nnrs_imp_expr_cases (induction e) Case
+        ; simpl ; intros e' eqq typ
+        ; try discriminate.
+        - Case "NNRSimpVar"%string.
+          match_destr_in eqq.
+          invcs eqq; simpl.
+          rewrite e.
+          unfold var in *.
+          rewrite inn.
+          rewrite lookup_update_eq_in; eauto.
+          apply lookup_in_domain in inn; trivial.
+        - Case "NNRSimpConst"%string.
+          destruct d0; try discriminate.
+          destruct l; try discriminate.
+          + invcs eqq; simpl; reflexivity.
+          + destruct d0; try discriminate.
+             destruct l; try discriminate.
+             invcs eqq; simpl.
+             unfold oflatten; simpl.
+            rewrite app_nil_r; trivial.
+        - Case "NNRSimpBinop"%string.
+          destruct b; try discriminate.
+          apply some_lift2 in eqq.
+          destruct eqq as [?[? eqq1[eqq2 ?]]]; subst.
+          simpl.
+          invcs typ.
+          invcs H3.
+          apply Coll_right_inv in H; subst.
+          specialize (IHe1 _ eqq1 H5).
+          specialize (IHe2 _ eqq2 H6).
+          unfold lift2P in *; simpl.
+          repeat match_option_in IHe1
+          ; simpl in *
+          ; try contradiction.
+          repeat match_option_in IHe2
+          ; simpl in *
+          ; try contradiction.
+
+          destruct d0; simpl in *; try contradiction
+          ; destruct d1; simpl in *; try contradiction
+          ; trivial.
+          destruct d2; simpl in *; try contradiction
+          ; destruct d3; simpl in *; try contradiction
+          ; trivial.
+          unfold bunion.
+          erewrite oflatten_app; eauto.
+        - Case "NNRSimpUnop"%string.
+          destruct u; simpl; try discriminate.
+          match_destr_in eqq.
+          invcs eqq.
+          invcs typ.
+          invcs H2.
+          apply Coll_right_inv in H.
+          rtype_equalizer; subst.
+          replace (nnrs_imp_expr_eval brand_relation_brands σc (update_first equiv_dec σ v d') e')
+            with (nnrs_imp_expr_eval brand_relation_brands σc σ e').
+          + 
+            case_eq (nnrs_imp_expr_eval brand_relation_brands σc σ e'); simpl; trivial.
+            intros ? eqq.
+            eapply nnrs_imp_expr_eval_preserves_types in eqq; eauto.
+            dtype_inverter.
+            rewrite oflatten_cons with (r':=nil); simpl; trivial.
+            rewrite app_nil_r; trivial.
+          + eapply nnrs_imp_expr_eval_same.
+            red; intros.
+            destruct (x == v).
+            * rewrite e in *; tauto.
+            * rewrite lookup_update_neq; eauto.
+      Qed.
+
+          Ltac disect_tac H stac
+    := 
+      unfold var in *
+      ; cut_to H; unfold domain in *; [ | solve[stac]..]
+      ; unfold lift2P in H
+      ; (repeat match_option_in H; try contradiction).
+
+  Ltac pcong
+    := solve[repeat (match goal with
+                     | [H: _ = _ |- _ ] => rewrite H in *; clear H
+                     end; try tauto)].
+
+  Ltac fuse_t stac
+    := repeat progress (
+                repeat rewrite in_app_iff in *
+                ; repeat
+                    match goal with
+                    | [H : ~ (_ \/ _ ) |- _ ] => apply not_or in H
+                    | [H : (_ \/ _ ) -> False |- _ ] => apply not_or in H
+                    | [H: _ /\ _ |- _ ] => destruct H
+                    | [ H : _ * _ |- _ ] => destruct H
+                    | [H: _::_ = _::_ |- _ ] => invcs H
+                    | [ H: domain (_ ++ _) = domain _ |- _ ] =>
+                      rewrite domain_app in H
+                      ; unfold domain in H
+                      ; symmetry in H; apply map_app_break in H
+                      ; destruct H as [? [?[?[??]]]]; subst; simpl in *
+                    | [ H: map (_ ++ _) = map _ |- _ ] =>
+                      rewrite map_app in H
+                      ; symmetry in H; apply map_app_break in H
+                      ; destruct H as [? [?[?[??]]]]; subst; simpl in *
+                    | [ H: _ :: _ = map _ ?x |- _ ] =>
+                      destruct x; try discriminate; simpl in H; invcs H
+                    | [ H: _ :: _ = domain ?x |- _ ] =>
+                      destruct x; try discriminate; simpl in H; invcs H
+                    | [H : ~ In _ (remove _ _ _) |- _ ] =>
+                      apply not_in_remove_impl_not_in in H; [| congruence]
+                    | [H : ?x ++ _ = ?y ++ _ |- _ ] =>
+                      let HH := fresh in
+                      assert (HH:domain y = domain x) by
+                          (unfold domain in *;
+                           try (intuition congruence)
+                           ; pcong)
+                      ; apply app_inv_head_domain in H;[clear HH|apply HH]
+
+                    | [ H: forall a b c, _ -> ?x1 :: ?dd :: ?x2 = _ ++ _ :: _ -> _ |- _] =>
+                      specialize (H (x1::nil) (snd dd) x2); simpl in H
+                      ; match dd with
+                        | (_,_) => idtac
+                        | _ => destruct dd
+                        end
+                      ; simpl in *
+                      ; cut_to H; [ | eauto 3 | reflexivity]
+                    end
+                ; simpl in *; trivial; intros; try subst; try contradiction; try solve [congruence | f_equal; congruence]).
+
+    Ltac fuse_tt := fuse_t ltac:(try tauto; try congruence).
+
+      Lemma nnrs_imp_stmt_unflatten_eval s s' v σc σ d :
+        nnrs_imp_stmt_unflatten s v = Some s' ->
+        forall Γc,
+          bindings_type σc Γc ->
+          forall Γ,
+            pd_bindings_type σ Γ ->
+            forall τ,
+              lookup equiv_dec σ v = Some d ->
+              lookup equiv_dec Γ v = Some (Coll (Coll τ)) ->
+              [ Γc ; Γ  ⊢ s ] ->
+              forall d',
+              lift2P flattens_to d d' ->
+              lift2P
+                (fun σ₁' σ₂' =>
+                   match lookup equiv_dec σ₁' v with
+                   | Some dd => 
+                     exists dd',
+                       σ₂' = update_first equiv_dec σ₁' v dd'
+                       /\ lift2P flattens_to dd dd'
+                   | None => False
+                   end
+                )
+                (nnrs_imp_stmt_eval brand_relation_brands σc s σ)
+                (nnrs_imp_stmt_eval brand_relation_brands σc s' (update_first equiv_dec σ v d')).
+      Proof.
+        intros eqq Γc σc_bt.
+        revert s' σ d eqq.
+        nnrs_imp_stmt_cases (induction s) Case
+        ; simpl ; intros s' σ d eqq Γ σ_bt τ σinn Γinn typ d' ft.
+        - Case "NNRSimpSkip"%string.
+          invcs eqq; simpl; intros.
+          unfold var in *.
+          rewrite σinn.
+          eauto.
+        - Case "NNRSimpSeq"%string.
+          apply some_lift2 in eqq.
+          destruct eqq as [?[? eqq1 [eqq2 ?]] ]; subst; simpl.
+          invcs typ.
+          specialize (IHs1 _ _ _ eqq1 _ σ_bt _ σinn Γinn H2 _ ft).
+          unfold lift2P in *.
+          do 3 (match_option_in IHs1; simpl in *
+                ; try contradiction).
+          destruct IHs1 as [dd' [? ft']].
+          subst.
+          generalize (nnrs_imp_stmt_eval_preserves_types _ σc_bt σ_bt H2 _ eqq)
+          ; intros p_bt.
+          eapply IHs2; eauto.
+        - Case "NNRSimpAssign"%string.
+          destruct (equiv_dec v0 v); unfold equiv, complement in *.
+          + subst; simpl in *.
+            apply some_lift in eqq.
+            destruct eqq as [? eqq ?]; subst.
+            invcs typ.
+            unfold equiv_dec, string_eqdec in *.
+            rewrite Γinn in H3.
+            invcs H3.
+            generalize (nnrs_imp_expr_unflatten_write_eval _ _ _ _ _
+                                                           eqq _ σc_bt _ σ_bt _ H2 _ _ σinn ft)
+            ; intros ft'.
+            simpl.
+            unfold lift2P in ft'.
+            unfold equiv_dec, string_eqdec in *.
+
+            repeat match_option_in ft'
+          ; simpl in *
+          ; try contradiction.
+            rewrite σinn.
+            simpl.
+            repeat rewrite lookup_update_eq_in.
+            * exists (Some d1).
+              repeat rewrite update_first_update_first_eq; simpl.
+              tauto.
+            * apply lookup_in_domain in σinn; trivial.
+            * apply lookup_in_domain in σinn; trivial.
+          + apply some_lift in eqq.
+             destruct eqq as [? eqq ?]; subst.
+             invcs typ.
+            rewrite (nnrs_imp_expr_unflatten_read_eval _ _ _ brand_relation_brands σc _ _ _
+                                                       eqq σinn ft).
+            simpl.
+            unfold equiv_dec, string_eqdec, var in *.
+            match_option; simpl; trivial.
+            rewrite lookup_update_neq by eauto.
+            match_option; simpl; trivial.
+            rewrite lookup_update_neq by eauto.
+            rewrite σinn.
+            exists d'.
+            split; trivial.
+            rewrite update_first_update_first_neq_swap; eauto.
+        - Case "NNRSimpLet"%string.
+          apply some_lift2 in eqq.
+          destruct eqq as [?[? eqq1 [eqq2 ?]] ]; subst; simpl.
+          invcs typ.
+          + simpl in eqq1.
+            apply some_lift in eqq1.
+            destruct eqq1 as [? eqq1 ?]; subst.
+            rewrite <- (nnrs_imp_expr_unflatten_read_eval _ _ _ brand_relation_brands σc _ _ _
+                                                            eqq1 σinn ft).
+            case_eq (nnrs_imp_expr_eval brand_relation_brands σc σ e₁); simpl; trivial
+            ; intros ? eveqq.
+            match_destr_in eqq2; unfold equiv, complement in *.
+            * subst.
+              invcs eqq2.
+              destruct (in_update_break_first _ σinn d')
+                as [?[? [? [eqq2 nin]]]]
+              ; subst.
+              rewrite eqq2.
+              generalize (nnrs_imp_stmt_eval_unused brand_relation_brands σc ((v, Some d0)::x) x2 x0 v d)
+              ; simpl ; intros HH1.
+              cut_to HH1; [| tauto].
+              generalize (nnrs_imp_stmt_eval_unused brand_relation_brands σc ((v, Some d0)::x) x2 x0 v d')
+              ; simpl ; intros HH2.
+              cut_to HH2; [| tauto].
+              unfold lift2P, var in *.
+              repeat match_option_in HH1
+              ; rewrite eqq0 in HH2
+              ; try contradiction
+              ; repeat match_option_in HH2
+              ; try contradiction.
+              apply nnrs_imp_stmt_eval_domain_stack in eqq.
+              apply nnrs_imp_stmt_eval_domain_stack in eqq3.
+              fuse_tt.
+              rewrite lookup_app.
+              rewrite lookup_nin_none; [|  unfold domain in *; congruence].
+              simpl.
+              destruct (equiv_dec s s); [| congruence].
+              exists o0.
+              rewrite update_app_nin; [|  unfold domain in *; congruence].
+              simpl.
+              destruct (equiv_dec s s); [| congruence].
+              specialize (HH1 ((s,o1)::x5) o2 x6); simpl in HH1.
+              cut_to HH1; [| unfold domain in *; congruence | trivial].
+              specialize (HH2 ((s,o)::x3) o0 x4); simpl in HH2.
+              cut_to HH2; [| unfold domain in *; congruence | trivial].
+              destruct HH1; subst.
+              fuse_tt.
+              split; trivial.
+            * assert (σ_bt_cons : pd_bindings_type ((v0, Some d0) :: σ) ((v0, τ0) :: Γ)).
+              {
+                econstructor; simpl; trivial.
+                split; trivial; intros.
+                invcs H.
+                eapply nnrs_imp_expr_eval_preserves_types  in eveqq; eauto.
+              } 
+              specialize (IHs _ ((v0, Some d0)::σ) d eqq2 ((v0, τ0) :: Γ) σ_bt_cons τ).
+              cut_to IHs; simpl; trivial; try solve [match_destr; congruence].
+              specialize (IHs _ ft).
+              simpl in IHs.
+              unfold var in *.
+              destruct (equiv_dec v v0); try congruence.
+              unfold lift2P in *.
+              do 2 match_option_in IHs
+              ; try contradiction.
+              generalize (nnrs_imp_stmt_eval_domain_stack eqq)
+              ; generalize (nnrs_imp_stmt_eval_domain_stack eqq0)
+              ; intros.
+              fuse_tt.
+              destruct (equiv_dec v s0); [congruence| ].
+              match_option_in IHs.
+              destruct IHs as [dd' [HH1 HH2]].
+              invcs HH1.
+              exists dd'; split; trivial.
+          + simpl in eqq1; invcs eqq1.
+            match_destr_in eqq2; unfold equiv, complement in *.
+            * subst.
+              invcs eqq2.
+              destruct (in_update_break_first _ σinn d')
+                as [?[? [? [eqq2 nin]]]]
+              ; subst.
+              rewrite eqq2.
+              generalize (nnrs_imp_stmt_eval_unused brand_relation_brands σc ((v, None)::x) x1 x0 v d)
+              ; simpl ; intros HH1.
+              cut_to HH1; [| tauto].
+              generalize (nnrs_imp_stmt_eval_unused brand_relation_brands σc ((v, None)::x) x1 x0 v d')
+              ; simpl ; intros HH2.
+              cut_to HH2; [| tauto].
+              unfold lift2P, var in *.
+              repeat match_option_in HH1
+              ; rewrite eqq0 in HH2
+              ; try contradiction
+              ; repeat match_option_in HH2
+              ; try contradiction.
+              apply nnrs_imp_stmt_eval_domain_stack in eqq.
+              apply nnrs_imp_stmt_eval_domain_stack in eqq1.
+              fuse_tt.
+              rewrite lookup_app.
+              rewrite lookup_nin_none; [|  unfold domain in *; congruence].
+              simpl.
+              destruct (equiv_dec s s); [| congruence].
+              exists o0.
+              rewrite update_app_nin; [|  unfold domain in *; congruence].
+              simpl.
+              destruct (equiv_dec s s); [| congruence].
+              specialize (HH1 ((s,o1)::x4) o2 x5); simpl in HH1.
+              cut_to HH1; [| unfold domain in *; congruence | trivial].
+              specialize (HH2 ((s,o)::x2) o0 x3); simpl in HH2.
+              cut_to HH2; [| unfold domain in *; congruence | trivial].
+              destruct HH1; subst.
+              fuse_tt.
+              split; trivial.
+            * assert (σ_bt_cons : pd_bindings_type ((v0, None) :: σ) ((v0, τ0) :: Γ)).
+              {
+                econstructor; simpl; trivial.
+                split; trivial; intros.
+                invcs H.
+              } 
+              specialize (IHs _ ((v0, None)::σ) d eqq2 ((v0, τ0) :: Γ) σ_bt_cons τ).
+              cut_to IHs; simpl; trivial; try solve [match_destr; congruence].
+              specialize (IHs _ ft).
+              simpl in IHs.
+              unfold var in *.
+              destruct (equiv_dec v v0); try congruence.
+              unfold lift2P in *.
+              do 2 match_option_in IHs
+              ; try contradiction.
+              generalize (nnrs_imp_stmt_eval_domain_stack eqq)
+              ; generalize (nnrs_imp_stmt_eval_domain_stack eqq0)
+              ; intros.
+              fuse_tt.
+              destruct (equiv_dec v s0); [congruence| ].
+              match_option_in IHs.
+              destruct IHs as [dd' [HH1 HH2]].
+              invcs HH1.
+              exists dd'; split; trivial.
+        - Case "NNRSimpFor"%string.
+          apply some_lift2 in eqq.
+          destruct eqq as [?[? eqq1 [eqq2 ?]] ]; subst; simpl.
+          invcs typ.
+          rewrite <- (nnrs_imp_expr_unflatten_read_eval _ _ _ brand_relation_brands σc _ _ _
+                                                        eqq1 σinn ft).
+          case_eq (nnrs_imp_expr_eval brand_relation_brands σc σ n); simpl; trivial
+          ; intros ? eveqq.
+          eapply nnrs_imp_expr_eval_preserves_types  in eveqq; eauto.
+          dtype_inverter.
+          invcs eveqq; rtype_equalizer; subst.
+          clear x n eqq1 H2.
+          revert σ Γ d d' σinn σ_bt H4 Γinn ft.
+          induction d0; intros σ Γ d d' σinn σ_bt typ Γinn ft; simpl; unfold var in *.
+          + rewrite σinn; eauto.
+          + invcs H1.
+            specialize (IHd0 H3); clear H3.
+            match_destr_in eqq2; unfold equiv, complement in *.
+            * subst.
+              invcs eqq2.
+              destruct (in_update_break_first _ σinn d')
+                as [?[? [? [eqq2 nin]]]]
+              ; subst.
+              rewrite eqq2.
+              clear eqq2.
+              generalize (nnrs_imp_stmt_eval_unused brand_relation_brands σc ((v, Some a)::x) x1 x0 v d)
+              ; simpl ; intros HH1.
+              cut_to HH1; [| tauto].
+              generalize (nnrs_imp_stmt_eval_unused brand_relation_brands σc ((v, Some a)::x) x1 x0 v d')
+              ; simpl ; intros HH2.
+              cut_to HH2; [| tauto].
+              unfold lift2P, var in *.
+              repeat match_option_in HH1
+              ; rewrite eqq0 in HH2
+              ; try contradiction
+              ; repeat match_option_in HH2
+              ; try contradiction.
+              generalize (nnrs_imp_stmt_eval_domain_stack eqq).
+              generalize (nnrs_imp_stmt_eval_domain_stack eqq1).
+              fuse_tt.
+              specialize (HH1 ((s,o)::x2) o0 x3); simpl in HH1.
+              cut_to HH1; [| unfold domain in *; congruence | trivial].
+              specialize (HH2 ((s,o1)::x4) o2 x5); simpl in HH2.
+              cut_to HH2; [| unfold domain in *; congruence | trivial].
+              destruct HH1; subst.
+              fuse_tt.
+              { eapply nnrs_imp_stmt_eval_preserves_types  in eqq; eauto.
+                - specialize (IHd0 (x4 ++ (s, o0) :: x5) Γ o0 o2).
+                  { cut_to IHd0; trivial.
+                - unfold lift2P in *.
+                  rewrite update_app_nin in IHd0; [ | unfold domain in *; congruence].
+                  simpl in IHd0.
+                  destruct (equiv_dec s s); [| congruence].
+                  trivial.
+                - rewrite lookup_app.
+                  rewrite lookup_nin_none; simpl.
+                  + destruct (equiv_dec s s); [| congruence]; trivial.
+                  + unfold domain in *; congruence.
+                - invcs eqq; auto.
+                  } 
+                - econstructor; simpl; trivial; split; trivial; intros ? eqqq; invcs eqqq; trivial.
+              }
+            * assert (σ_bt_cons : pd_bindings_type ((v0, Some a) :: σ) ((v0, τ0) :: Γ)).
+              {
+                econstructor; simpl; trivial.
+                split; trivial; intros.
+                invcs H; trivial.
+              } 
+              specialize (IHs _ ((v0, Some a)::σ) d eqq2 ((v0, τ0) :: Γ) σ_bt_cons τ).
+              cut_to IHs; simpl; trivial; try solve [match_destr; congruence].
+              specialize (IHs _ ft).
+              simpl in IHs.
+              unfold var in *.
+              destruct (equiv_dec v v0); try congruence.
+              unfold lift2P in *.
+              do 2 match_option_in IHs
+              ; try contradiction.
+              generalize (nnrs_imp_stmt_eval_domain_stack eqq)
+              ; generalize (nnrs_imp_stmt_eval_domain_stack eqq0)
+              ; intros.
+              fuse_tt.
+              destruct (equiv_dec v s0); [congruence| ].
+              match_option_in IHs; try contradiction.
+              destruct IHs as [dd' [HH1 HH2]].
+              invcs HH1.
+              clear H3.
+              generalize (nnrs_imp_stmt_eval_preserves_types _ σc_bt σ_bt_cons typ _ eqq)
+              ; intros p_bt.
+              invcs p_bt.
+              specialize (IHd0 p1 Γ o1 dd').
+              cut_to IHd0; trivial.
+        - Case "NNRSimpIf"%string.
+          unfold lift3 in eqq.
+          repeat match_option_in eqq.
+          invcs eqq; simpl in *.
+          invcs typ.
+          rewrite <- (nnrs_imp_expr_unflatten_read_eval _ _ _ brand_relation_brands σc _ _ _
+                                                     eqq0 σinn ft).
+          match_option; simpl; trivial.
+          destruct d0; simpl; trivial.
+          destruct b; eauto.
+        - Case "NNRSimpEither"%string.
+          unfold lift3 in eqq.
+          repeat match_option_in eqq.
+          invcs eqq; simpl in *.
+          invcs typ.
+          rewrite <- (nnrs_imp_expr_unflatten_read_eval _ _ _ brand_relation_brands σc _ _ _
+                                                     eqq0 σinn ft).
+          match_option; simpl; trivial.
+          eapply nnrs_imp_expr_eval_preserves_types  in eqq; eauto.
+          destruct d0; simpl; trivial
+          ; invcs eqq; rtype_equalizer; subst.
+          + match_destr_in eqq1; unfold equiv, complement in *.
+            * subst.
+              invcs eqq1.
+              destruct (in_update_break_first _ σinn d')
+                as [?[? [? [eqq1 nin]]]]
+              ; subst.
+              rewrite eqq1.
+              generalize (nnrs_imp_stmt_eval_unused brand_relation_brands σc ((v, Some d0)::x) x0 n1 v d)
+              ; simpl ; intros HH1.
+              cut_to HH1; [| tauto].
+              generalize (nnrs_imp_stmt_eval_unused brand_relation_brands σc ((v, Some d0)::x) x0 n1 v d')
+              ; simpl ; intros HH2.
+              cut_to HH2; [| tauto].
+              unfold lift2P, var in *.
+              repeat match_option_in HH1
+              ; rewrite eqq3 in HH2
+              ; try contradiction
+              ; repeat match_option_in HH2
+              ; try contradiction.
+              apply nnrs_imp_stmt_eval_domain_stack in eqq.
+              apply nnrs_imp_stmt_eval_domain_stack in eqq4.
+              fuse_tt.
+              rewrite lookup_app.
+              rewrite lookup_nin_none; [|  unfold domain in *; congruence].
+              simpl.
+              destruct (equiv_dec s s); [| congruence].
+              exists o0.
+              rewrite update_app_nin; [|  unfold domain in *; congruence].
+              simpl.
+              destruct (equiv_dec s s); [| congruence].
+              specialize (HH1 ((s,o1)::x3) o2 x4); simpl in HH1.
+              cut_to HH1; [| unfold domain in *; congruence | trivial].
+              specialize (HH2 ((s,o)::x1) o0 x2); simpl in HH2.
+              cut_to HH2; [| unfold domain in *; congruence | trivial].
+              destruct HH1; subst.
+              fuse_tt.
+              split; trivial.
+            * assert (σ_bt_cons : pd_bindings_type ((v0, Some d0) :: σ) ((v0, τl) :: Γ)).
+              {
+                econstructor; simpl; trivial.
+                split; trivial; intros.
+                invcs H; trivial.
+              } 
+              specialize (IHs1 _ ((v0, Some d0)::σ) d eqq1 ((v0, τl) :: Γ) σ_bt_cons τ).
+              cut_to IHs1; simpl; trivial; try solve [match_destr; congruence].
+              specialize (IHs1 _ ft).
+              simpl in IHs1.
+              unfold var in *.
+              destruct (equiv_dec v v0); try congruence.
+              unfold lift2P in *.
+              do 2 match_option_in IHs1
+              ; try contradiction.
+              generalize (nnrs_imp_stmt_eval_domain_stack eqq)
+              ; generalize (nnrs_imp_stmt_eval_domain_stack eqq3)
+              ; intros.
+              fuse_tt.
+              destruct (equiv_dec v s); [congruence| ].
+              match_option_in IHs1.
+              destruct IHs1 as [dd' [HH1 HH2]].
+              invcs HH1.
+              exists dd'; split; trivial. 
+          + match_destr_in eqq2; unfold equiv, complement in *.
+            * subst.
+              invcs eqq2.
+              destruct (in_update_break_first _ σinn d')
+                as [?[? [? [eqq2 nin]]]]
+              ; subst.
+              rewrite eqq2.
+              generalize (nnrs_imp_stmt_eval_unused brand_relation_brands σc ((v, Some d0)::x) x0 n2 v d)
+              ; simpl ; intros HH1.
+              cut_to HH1; [| tauto].
+              generalize (nnrs_imp_stmt_eval_unused brand_relation_brands σc ((v, Some d0)::x) x0 n2 v d')
+              ; simpl ; intros HH2.
+              cut_to HH2; [| tauto].
+              unfold lift2P, var in *.
+              repeat match_option_in HH1
+              ; rewrite eqq3 in HH2
+              ; try contradiction
+              ; repeat match_option_in HH2
+              ; try contradiction.
+              apply nnrs_imp_stmt_eval_domain_stack in eqq.
+              apply nnrs_imp_stmt_eval_domain_stack in eqq4.
+              fuse_tt.
+              rewrite lookup_app.
+              rewrite lookup_nin_none; [|  unfold domain in *; congruence].
+              simpl.
+              destruct (equiv_dec s s); [| congruence].
+              exists o0.
+              rewrite update_app_nin; [|  unfold domain in *; congruence].
+              simpl.
+              destruct (equiv_dec s s); [| congruence].
+              specialize (HH1 ((s,o1)::x3) o2 x4); simpl in HH1.
+              cut_to HH1; [| unfold domain in *; congruence | trivial].
+              specialize (HH2 ((s,o)::x1) o0 x2); simpl in HH2.
+              cut_to HH2; [| unfold domain in *; congruence | trivial].
+              destruct HH1; subst.
+              fuse_tt.
+              split; trivial.
+            * assert (σ_bt_cons : pd_bindings_type ((v1, Some d0) :: σ) ((v1, τr) :: Γ)).
+              {
+                econstructor; simpl; trivial.
+                split; trivial; intros.
+                invcs H; trivial.
+              } 
+              specialize (IHs2 _ ((v1, Some d0)::σ) d eqq2 ((v1, τr) :: Γ) σ_bt_cons τ).
+              cut_to IHs2; simpl; trivial; try solve [match_destr; congruence].
+              specialize (IHs2 _ ft).
+              simpl in IHs2.
+              unfold var in *.
+              destruct (equiv_dec v v1); try congruence.
+              unfold lift2P in *.
+              do 2 match_option_in IHs2
+              ; try contradiction.
+              generalize (nnrs_imp_stmt_eval_domain_stack eqq)
+              ; generalize (nnrs_imp_stmt_eval_domain_stack eqq3)
+              ; intros.
+              fuse_tt.
+              destruct (equiv_dec v s); [congruence| ].
+              match_option_in IHs2.
+              destruct IHs2 as [dd' [HH1 HH2]].
+              invcs HH1.
+              exists dd'; split; trivial. 
+      Qed.
+
+  End eval.
+  
+  Section typ.
+
+    Lemma nnrs_imp_expr_unflatten_init_type {e e':nnrs_imp_expr}:
+      nnrs_imp_expr_unflatten_init e = Some e' ->
+      forall {Γc Γ τ},
+        [ Γc ; Γ  ⊢ e ▷ Coll (Coll τ) ]  ->
+        [ Γc ; Γ  ⊢ e' ▷ Coll τ ].
+    Proof.
+      revert e'.
+      nnrs_imp_expr_cases (induction e) Case
+      ; simpl ; intros e' eqq Γc Γ τ typ
+      ; try discriminate.
+      - Case "NNRSimpConst"%string.
+        destruct d; simpl in *
+        ; invcs eqq.
+        invcs typ.
+        invcs H2.
+        apply Coll_right_inv in H1; subst.
+        destruct l; invcs H0; simpl.
+        + repeat econstructor.
+        + simpl in H3; invcs H3.
+          invcs H2; rtype_equalizer; subst.
+          destruct d; try discriminate.
+          destruct l; try discriminate.
+            invcs H1.
+            econstructor.
+            rewrite <- H.
+            econstructor; trivial.
+        - Case "NNRSimpBinop"%string.
+          destruct b; try discriminate.
+          apply some_lift2 in eqq.
+          destruct eqq as [?[? eqq1[eqq2 ?]]]; subst.
+          invcs typ.
+          invcs H3.
+          apply Coll_right_inv in H; subst.
+          econstructor; eauto.
+          econstructor.
+        - Case "NNRSimpUnop"%string.
+          destruct u; try discriminate.
+          destruct e; try discriminate.
+          + destruct d; try discriminate.
+            invcs typ.
+            invcs H2.
+            apply Coll_right_inv in H; subst.
+            invcs eqq; trivial.
+          + destruct u; try discriminate.
+            invcs eqq.
+            invcs typ.
+            invcs H2.
+            apply Coll_right_inv in H; subst.
+            trivial.
+    Qed.
+          
+    Lemma nnrs_imp_expr_unflatten_read_type e e' v :
+      nnrs_imp_expr_unflatten_read e v = Some e' ->
+      forall {Γc Γ τo},
+        [ Γc ; Γ  ⊢ e ▷ τo]  ->
+        forall τ,
+          lookup equiv_dec Γ v = Some (Coll τ) ->
+          [ Γc ; (update_first equiv_dec Γ v τ)   ⊢ e' ▷ τo ].
+    Proof.
+      revert e'.
+      nnrs_imp_expr_cases (induction e) Case
+        ; simpl ; intros e' eqq Γc Γ τo typ τ inn.
+        - Case "NNRSimpGetConstant"%string.
+          invcs eqq.
+          invcs typ.
+          econstructor; trivial.
+        - Case "NNRSimpVar"%string.
+          match_destr_in eqq.
+          invcs eqq; simpl.
+          invcs typ.
+          econstructor.
+          rewrite lookup_update_neq; trivial.
+          eauto.
+        - Case "NNRSimpConst"%string.
+          invcs eqq; simpl; trivial.
+          invcs typ.
+          econstructor; trivial.
+        - Case "NNRSimpBinop"%string.
+          apply some_lift2 in eqq.
+          destruct eqq as [?[? eqq1[eqq2 ?]]]; subst.
+          invcs typ.
+          econstructor; eauto.
+        - Case "NNRSimpUnop"%string.
+          invcs typ.
+          destruct u
+          ; try solve [apply some_lift in eqq
+          ; destruct eqq as [eqq1 eqq2]
+          ; subst; simpl
+          ; econstructor; eauto].
+          destruct e
+          ; try solve [apply some_lift in eqq
+                       ; destruct eqq as [eqq1 eqq2]
+                       ; subst; simpl
+                       ; econstructor; eauto].
+          invcs H2.
+          invcs H4.
+          match_destr_in eqq.
+          + invcs eqq; simpl.
+            rewrite e in *.
+            unfold var in *.
+            rewrite inn in H1; invcs H1; rtype_equalizer.
+            apply Coll_right_inv in H0; subst.
+            econstructor.
+            rewrite lookup_update_eq_in; try congruence.
+            apply lookup_in_domain in inn; trivial.
+          + invcs eqq; simpl.
+            econstructor; econstructor.
+            rewrite lookup_update_neq; eauto.
+        - Case "NNRSimpGroupBy"%string.
+          apply some_lift in eqq.
+          destruct eqq as [??]; subst; simpl.
+          invcs typ.
+          econstructor; trivial.
+          eauto.
+    Qed.
+
+    Lemma nnrs_imp_expr_unflatten_write_type e e' v :
+      nnrs_imp_expr_unflatten_write e v = Some e' ->
+      forall {Γc Γ τo},
+        [ Γc ; Γ  ⊢ e ▷ Coll (Coll τo)]  ->
+        forall τ,
+          lookup equiv_dec Γ v = Some (Coll τ) ->
+          [ Γc ; (update_first equiv_dec Γ v τ)   ⊢ e' ▷ Coll τo ].
+    Proof.
+      revert e'.
+      nnrs_imp_expr_cases (induction e) Case
+      ; simpl ; intros e' eqq Γc Γ τo typ τ inn
+      ; try discriminate.
+        - Case "NNRSimpVar"%string.
+          match_destr_in eqq.
+          rewrite e in *; clear v0 e.
+          invcs eqq; simpl.
+          invcs typ.
+          rewrite inn in H1.
+          invcs H1.
+          apply Coll_right_inv in H0; subst.
+          econstructor.
+          rewrite lookup_update_eq_in; eauto.
+          apply lookup_in_domain in inn; trivial.
+        - Case "NNRSimpConst"%string.
+          invcs typ.
+          destruct d; simpl; try discriminate.
+          destruct l; simpl; try discriminate.
+          + invcs eqq.
+            econstructor.
+            repeat econstructor.
+          + destruct d; simpl; try discriminate.
+             destruct l; simpl; try discriminate.
+             invcs eqq.
+             econstructor.
+             simpl in H1.
+             invcs H1.
+             apply Coll_right_inv in H0; subst.
+             invcs H2; trivial.
+        - Case "NNRSimpBinop"%string.
+          destruct b; try discriminate.
+          apply some_lift2 in eqq.
+          destruct eqq as [?[? eqq1[eqq2 ?]]]; subst.
+          invcs typ.
+          invcs H3.
+          apply Coll_right_inv in H; subst.
+          econstructor; eauto.
+          econstructor.
+        - Case "NNRSimpUnop"%string.
+          invcs typ.
+          destruct u; try discriminate.
+          match_destr_in eqq.
+          invcs eqq.
+          invcs H2.
+          apply Coll_right_inv in H; subst.
+          apply (nnrs_imp_expr_type_update_first_irrelevant Γc nil)
+          ; simpl; tauto.
+    Qed.
+
+    Lemma nnrs_imp_stmt_unflatten_type s s' v :
+      nnrs_imp_stmt_unflatten s v = Some s' ->
+      forall {Γc Γ},
+        [ Γc ; Γ  ⊢ s]  ->
+        forall τ,
+          lookup equiv_dec Γ v = Some (Coll (Coll τ)) ->
+          [ Γc ; (update_first equiv_dec Γ v (Coll τ))   ⊢ s'].
+    Proof.
+      revert s'
+      ; nnrs_imp_stmt_cases (induction s) Case
+      ; simpl in *; intros s' eqq Γc Γ typ τ inn.
+      - Case "NNRSimpSkip"%string.
+        invcs eqq.
+        econstructor.
+      - Case "NNRSimpSeq"%string.
+        apply some_lift2 in eqq.
+        destruct eqq as [?[? eqq1[eqq2 ?]]]; subst.
+        invcs typ.
+        econstructor; eauto.
+      - Case "NNRSimpAssign"%string.
+        apply some_lift in eqq.
+        destruct eqq as [??]; subst; simpl.
+        invcs typ.
+        match_destr_in e; unfold equiv, complement in *.
+        + subst.
+          unfold equiv_dec, string_eqdec in *.
+          rewrite inn in H3.
+          invcs H3.
+          econstructor.
+          * eapply nnrs_imp_expr_unflatten_write_type in e; eauto.
+          * rewrite lookup_update_eq_in; eauto.
+            apply lookup_in_domain in inn; trivial.
+        + econstructor.
+          * eapply nnrs_imp_expr_unflatten_read_type in e; eauto.
+          * rewrite lookup_update_neq; eauto.
+      - Case "NNRSimpLet"%string.
+        apply some_lift2 in eqq.
+        destruct eqq as [?[? eqq1[eqq2 ?]]]; subst.
+        invcs typ; simpl in *.
+        + apply some_lift in eqq1.
+           destruct eqq1 as [? eqq1 ?]; subst; simpl.
+           econstructor.
+          * eapply nnrs_imp_expr_unflatten_read_type in eqq1; eauto.
+          * { match_destr_in eqq2; unfold equiv, complement in *.
+              - invcs eqq2.
+                apply (nnrs_imp_stmt_type_update_first_irrelevant Γc ((v, τ0) :: nil))
+                ; simpl; tauto.
+              - specialize (IHs _ eqq2 _ _ H4).
+                simpl in IHs.
+                unfold var in *.
+                destruct (equiv_dec v v0); [congruence | ].
+                eauto.
+            }
+        + invcs eqq1.
+          match_destr_in eqq2; unfold equiv, complement in *.
+          * invcs eqq2.
+            econstructor; trivial.
+            apply (nnrs_imp_stmt_type_update_first_irrelevant Γc ((v, τ0) :: nil))
+                ; simpl; tauto.
+          * { econstructor.
+              - rewrite <- (nnrs_imp_stmt_unflatten_var_usage eqq2); trivial.
+              - specialize (IHs _ eqq2 _ _ H4).
+                simpl in IHs.
+                unfold var in *.
+                destruct (equiv_dec v v0); [congruence | ].
+                eauto.
+            }
+      - Case "NNRSimpFor"%string.
+        apply some_lift2 in eqq.
+        destruct eqq as [?[? eqq1[eqq2 ?]]]; subst.
+        invcs typ.
+        eapply nnrs_imp_expr_unflatten_read_type in eqq1; eauto.
+        econstructor; trivial; eauto.
+        match_destr_in eqq2; unfold equiv, complement in *.
+        + invcs eqq2.
+          apply (nnrs_imp_stmt_type_update_first_irrelevant Γc ((v, τ0) :: nil))
+          ; simpl; tauto.
+        +  specialize (IHs _ eqq2 _ _ H4).
+           simpl in IHs.
+           unfold var in *.
+           destruct (equiv_dec v v0); [congruence | ].
+           eauto.
+      - Case "NNRSimpIf"%string.
+        unfold lift3 in eqq.
+        repeat match_option_in eqq.
+        invcs eqq; simpl.
+        invcs typ.
+        eapply nnrs_imp_expr_unflatten_read_type in eqq0; eauto.
+        econstructor; eauto.
+      - Case "NNRSimpEither"%string.
+        unfold lift3 in eqq.
+        repeat match_option_in eqq.
+        invcs eqq; simpl.
+        invcs typ.
+        eapply nnrs_imp_expr_unflatten_read_type in eqq0; eauto.
+        econstructor; eauto.
+        + match_destr_in eqq1; unfold equiv, complement in *.
+          * invcs eqq1.
+            apply (nnrs_imp_stmt_type_update_first_irrelevant Γc ((v, τl) :: nil))
+            ; simpl; tauto.
+          * specialize (IHs1 _ eqq1 _ _ H6).
+            simpl in IHs1.
+            unfold var in *.
+            destruct (equiv_dec v v0); [congruence | ].
+            eauto.
+        + match_destr_in eqq2; unfold equiv, complement in *.
+          * invcs eqq2.
+            apply (nnrs_imp_stmt_type_update_first_irrelevant Γc ((v, τr) :: nil))
+            ; simpl; tauto.
+          * specialize (IHs2 _ eqq2 _ _ H7).
+            simpl in IHs2.
+            unfold var in *.
+            destruct (equiv_dec v v1); [congruence | ].
+            eauto.
+    Qed.
+
+  End typ.
+
+  Section type_enrich.
+
+    Lemma nnrs_imp_expr_unflatten_read_enrich_type {e e' v} :
+      nnrs_imp_expr_unflatten_read e v = Some e' ->
+      forall {Γc Γ τo},
+        [ Γc ; Γ  ⊢ e ▷ τo]  ->
+        forall τ,
+          In v (nnrs_imp_expr_free_vars e) ->
+          lookup equiv_dec Γ v = Some τ ->
+          exists τ', τ = Coll (Coll τ').
+    Proof.
+      revert e'.
+      nnrs_imp_expr_cases (induction e) Case
+      ; simpl ; intros e' eqq Γc Γ τo typ τ inn1 inn2
+      ; try contradiction.
+      - Case "NNRSimpVar"%string.
+        match_destr_in eqq.
+        intuition.
+      - Case "NNRSimpBinop"%string.
+        apply some_lift2 in eqq.
+        destruct eqq as [?[? eqq1[eqq2 ?]]]; subst.
+        invcs typ.
+        rewrite in_app_iff in inn1.
+        destruct inn1 as [inn1|inn1]; eauto.
+      - Case "NNRSimpUnop"%string.
+        invcs typ.
+          destruct u
+          ; try solve [apply some_lift in eqq
+                     ; destruct eqq as [eqq1 eqq2]
+                     ; subst; simpl
+                     ; invcs H2; eauto].
+          invcs H2.
+          destruct e
+          ; try solve [apply some_lift in eqq
+                     ; destruct eqq as [eqq1 eqq2]
+                     ; subst; simpl; eauto].
+          simpl in inn1.
+          match_destr_in eqq; [ | intuition congruence].
+          invcs eqq.
+          invcs H4.
+          intuition; subst.
+          rewrite H1 in inn2.
+          invcs inn2.
+          eauto.
+      - Case "NNRSimpGroupBy"%string.
+        apply some_lift in eqq.
+        destruct eqq as [? eqq ?].
+        subst; simpl.
+        invcs typ.
+        eauto.
+    Qed.
+
+    Lemma nnrs_imp_stmt_unflatten_read_out_type s s' v :
+      nnrs_imp_stmt_unflatten s v = Some s' ->
+      nnrs_imp_stmt_read_out s v = true ->
+      forall {Γc Γ},
+        [ Γc ; Γ  ⊢ s]  ->
+        forall τ,
+          lookup equiv_dec Γ v = Some τ ->
+          exists τ', τ = Coll (Coll τ').
+    Proof.
+      revert s'
+      ; nnrs_imp_stmt_cases (induction s) Case
+      ; simpl in *; intros s' eqq_un eqq_ro Γc Γ typ τ inn
+      ; unfold nequiv_decb, equiv_decb in *.
+      - Case "NNRSimpSkip"%string.
+        discriminate.
+      - Case "NNRSimpSeq"%string.
+        apply orb_true_elim in eqq_ro.
+        invcs typ.
+        apply some_lift2 in eqq_un.
+        destruct eqq_un as [?[? eqq1[eqq2 ?]]]; subst.
+        intuition eauto.
+      - Case "NNRSimpAssign"%string.
+        invcs typ.
+        apply some_lift in eqq_un.
+        destruct eqq_un as [? eqq ?].
+        subst; simpl.
+        match_destr_in eqq_ro.
+        simpl in *.
+        eapply nnrs_imp_expr_unflatten_read_enrich_type; eauto.
+        apply nnrs_imp_expr_may_use_free_vars; auto.
+      - Case "NNRSimpLet"%string.
+        apply orb_true_elim in eqq_ro.
+        apply some_lift2 in eqq_un.
+        destruct eqq_un as [?[? eqq1[eqq2 ?]]]; subst.
+        destruct eqq_ro.
+        + destruct o; try discriminate.
+          invcs typ.
+          simpl in eqq1.
+          apply some_lift in eqq1.
+          destruct eqq1 as [? eqq ?]; subst.
+          eapply nnrs_imp_expr_unflatten_read_enrich_type; eauto.
+          apply nnrs_imp_expr_may_use_free_vars; auto.
+        + match_destr_in e; simpl in e.
+          invcs typ; eapply IHs; eauto
+          ; simpl
+          ; match_destr
+          ; congruence.
+      - Case "NNRSimpFor"%string.
+        apply orb_true_elim in eqq_ro.
+        apply some_lift2 in eqq_un.
+        destruct eqq_un as [?[? eqq1[eqq2 ?]]]; subst.
+        invcs typ.
+        destruct eqq_ro.
+        + eapply nnrs_imp_expr_unflatten_read_enrich_type; eauto.
+          apply nnrs_imp_expr_may_use_free_vars; auto.
+        + match_destr_in eqq2.
+          simpl in e.
+          eapply IHs; eauto.
+          simpl; match_destr; congruence.
+      - unfold lift3 in eqq_un; repeat match_option_in eqq_un.
+        invcs eqq_un; subst.
+        invcs typ.
+        apply orb_true_elim in eqq_ro.
+        destruct eqq_ro as [eqq_ro | eqq_ro].
+        + apply orb_true_elim in eqq_ro.
+          destruct eqq_ro as [eqq_ro | eqq_ro].
+          * eapply nnrs_imp_expr_unflatten_read_enrich_type; eauto.
+            apply nnrs_imp_expr_may_use_free_vars; auto.
+          * eauto.
+        + eauto.
+      - unfold lift3 in eqq_un; repeat match_option_in eqq_un.
+        invcs eqq_un; subst.
+        invcs typ.
+        apply orb_true_elim in eqq_ro.
+        destruct eqq_ro as [eqq_ro | eqq_ro].
+        + apply orb_true_elim in eqq_ro.
+          destruct eqq_ro as [eqq_ro | eqq_ro].
+          * eapply nnrs_imp_expr_unflatten_read_enrich_type; eauto.
+            apply nnrs_imp_expr_may_use_free_vars; auto.
+          * match_destr_in eqq_ro.
+            eapply IHs1; eauto.
+            simpl; match_destr; congruence.
+        + match_destr_in eqq_ro.
+            eapply IHs2; eauto.
+            simpl; match_destr; congruence.
+    Qed.
+
+  End type_enrich.
+
+  Section unflatten_safe.
+
+    Lemma nnrs_imp_stmt_unflatten_safe_eval s s' v σc σ d :
+        nnrs_imp_stmt_unflatten_safe s v = Some s' ->
+        forall Γc,
+          bindings_type σc Γc ->
+          forall Γ,
+            pd_bindings_type σ Γ ->
+            forall τ,
+              lookup equiv_dec σ v = Some d ->
+              lookup equiv_dec Γ v = Some τ ->
+              [ Γc ; Γ  ⊢ s ] ->
+              forall d',
+                lift2P flattens_to d d' ->
+              lift2P
+                (fun σ₁' σ₂' =>
+                   match lookup equiv_dec σ₁' v with
+                   | Some dd => 
+                     exists dd',
+                       σ₂' = update_first equiv_dec σ₁' v dd'
+                       /\ lift2P flattens_to dd dd'
+                   | None => False
+                   end
+                )
+                (nnrs_imp_stmt_eval brand_relation_brands σc s σ)
+                (nnrs_imp_stmt_eval brand_relation_brands σc s' (update_first equiv_dec σ v d')).
+    Proof.
+      unfold nnrs_imp_stmt_unflatten_safe.
+      intros eqq1 Γc Γc_bt Γ Γ_bt τ inn1 inn2 typ; intros.
+      match_case_in eqq1; intros eqq2; rewrite eqq2 in eqq1; try discriminate.
+      intros.
+      destruct (nnrs_imp_stmt_unflatten_read_out_type _ _ _ eqq1 eqq2 typ _ inn2)
+      ; subst.
+      eapply nnrs_imp_stmt_unflatten_eval; eauto.
+    Qed.
+    
+    Lemma nnrs_imp_stmt_unflatten_safe_type s s' v :
+      nnrs_imp_stmt_unflatten_safe s v = Some s' ->
+      forall {Γc Γ},
+        [ Γc ; Γ  ⊢ s]  ->
+        forall τ,
+          lookup equiv_dec Γ v = Some τ ->
+        exists τ',
+          [ Γc ; (update_first equiv_dec Γ v (Coll τ'))   ⊢ s']
+          /\  τ = Coll (Coll τ').
+    Proof.
+      unfold nnrs_imp_stmt_unflatten_safe.
+      intros eqq1 Γc Γ typ τ inn.
+      match_case_in eqq1; intros eqq2; rewrite eqq2 in eqq1; try discriminate.
+      destruct (nnrs_imp_stmt_unflatten_read_out_type _ _ _ eqq1 eqq2 typ _ inn)
+      ; subst.
+      econstructor; split; try reflexivity.
+      eapply nnrs_imp_stmt_unflatten_type; eauto.
+    Qed.
+
+    Lemma nnrs_imp_stmt_unflatten_safe_var_usage {s s' v}:
+        nnrs_imp_stmt_unflatten_safe s v = Some s' ->
+        forall v',
+          nnrs_imp_stmt_var_usage s v' = nnrs_imp_stmt_var_usage s' v'.
+    Proof.
+      unfold nnrs_imp_stmt_unflatten_safe.
+      intros eqq1; intros.
+      match_case_in eqq1; intros eqq2; rewrite eqq2 in eqq1; try discriminate.
+      eapply nnrs_imp_stmt_unflatten_var_usage; eauto.
+    Qed.
+
+  End unflatten_safe.
+
+  
+End TNNRSimpUnflatten.
